theories/typing/adequacy.v
@@ -33,10 +33,10 @@ Definition initial_thread_state (main : loc) : thread_state := {|
   ts_alloc_failure := false;
 |}.
 
-Definition initial_state (fns : gmap loc function) (gs : gmap loc mbyte) (bs : allocs) :=
-  {| st_heap := (λ b, (RSt 0%nat, b) ) <$> gs;
+Definition initial_state (fns : gmap loc function) :=
+  {| st_heap := ∅;
      st_fntbl := fns;
-     st_allocs := bs;
+     st_allocs := ∅;
      st_alloc_failure := false; |}.
 
 Lemma wp_to_typed_stmt `{!typeG Σ} (ts : thread_state) v':
@@ -58,27 +58,26 @@ Definition main_type `{!typeG Σ} (P : iProp Σ) :=
   fn(∀ () : (); P) → ∃ () : (), int i32; True.
 
 (** * The main adequacy lemma *)
-Lemma refinedc_adequacy Σ `{!typePreG Σ} (thread_mains : list loc) (fns : gmap loc function) (gs : gmap loc mbyte) (bs : allocs) n t2 σ2 κs:
-  blocks_used_agree (initial_state fns gs bs).(st_heap) (initial_state fns gs bs).(st_allocs) →
+Lemma refinedc_adequacy Σ `{!typePreG Σ} (thread_mains : list loc) (fns : gmap loc function) (gls : list loc) (gvs : list lang.val) n t2 σ2 κs σ:
+  alloc_new_blocks (initial_state fns) gls gvs σ →
   (∀ {HtypeG : typeG Σ}, ∃ gl gt,
   let Hglobals : globalG Σ := {| global_locs := gl; global_initialized_types := gt; |} in
-    ([∗ map] k↦qs∈gs, heap_mapsto_mbyte k 1 qs) -∗
-    ([∗ map] k↦qs∈bs, allocs_entry k qs) -∗
+    ([∗ list] l; v ∈ gls; gvs, l ↦ v) -∗
     ([∗ map] k↦qs∈fns, fntbl_entry k qs) ={⊤}=∗
       [∗ list] main ∈ thread_mains, ∃ P, main ◁ᵥ main @ function_ptr (main_type P) ∗ P) →
-  nsteps (Λ := stmt_lang) n (initial_thread_state <$> thread_mains, initial_state fns gs bs) κs (t2, σ2) →
+  nsteps (Λ := stmt_lang) n (initial_thread_state <$> thread_mains, σ) κs (t2, σ2) →
   ∀ e2, e2 ∈ t2 → not_stuck e2 σ2.
 Proof.
-  move => Hvalid Hwp. apply: wp_strong_adequacy. move => ?.
-  set h := to_heap ((λ b, (RSt 0%nat, b)) <$> gs).
-  iMod (own_alloc (● h ⋅ ◯ h)) as (γh) "[Hh Hm]" => //.
-  { apply auth_both_valid_discrete. split => //. eauto using to_heap_valid. }
+  move => Hnew Hwp. apply: wp_strong_adequacy. move => ?.
+  set h := to_heap ∅.
+  iMod (own_alloc (● h ⋅ ◯ h)) as (γh) "[Hh _]" => //.
+  { apply auth_both_valid_discrete. split => //. }
   set f := to_fntbl fns.
   iMod (own_alloc (● f ⋅ ◯ f)) as (γf) "[Hf Hfm]" => //.
   { apply auth_both_valid_discrete. split => //. eauto using to_fntbl_valid. }
-  set b := to_allocs bs.
-  iMod (own_alloc (● b ⋅ ◯ b)) as (γb) "[Hb #Hbm]" => //.
-  { apply auth_both_valid_discrete. split => //. eauto using to_allocs_valid. }
+  set b := to_allocs ∅.
+  iMod (own_alloc (● b ⋅ ◯ b)) as (γb) "[Hb _]" => //.
+  { apply auth_both_valid_discrete. split => //. }
 
   set (HheapG := HeapG _ _ γh _ γb _ γf).
   set (HrefinedCG := RefinedCG _ _ HheapG).
@@ -86,23 +85,9 @@ Proof.
   move: (Hwp HtypeG) => {Hwp} [gl [gt]].
   set (Hglobals := {| global_locs := gl; global_initialized_types := gt; |}).
   move => Hwp.
-  iMod (Hwp with "[Hm] [] [Hfm]") as "Hmains". {
-    rewrite /h => {h Hwp Hvalid}.
-    iInduction (gs) as [|i ????] "IH" using map_ind => //.
-    iApply big_sepM_insert => //.
-    rewrite fmap_insert to_heap_insert insert_singleton_op. 2: by apply lookup_to_heap_None; simplify_map_eq.
-    rewrite heap_mapsto_mbyte_eq /heap_mapsto_mbyte_def /=.
-    iDestruct "Hm" as "[$ Hm]".
-    by iApply "IH".
-  } {
-    rewrite /b => {b Hwp Hvalid}.
-    iInduction (bs) as [|??? HNone] "IH" using map_ind => //.
-    iApply big_sepM_insert => //. rewrite /to_allocs fmap_insert.
-    rewrite (insert_singleton_op); last by rewrite lookup_fmap HNone.
-    rewrite allocs_entry_eq. iDestruct "Hbm" as "[$ Hfm]".
-    by iApply "IH".
-  } {
-    rewrite /f => {f Hwp Hvalid}.
+  iMod (heap_alloc_new_blocks_upd with "[Hh Hf Hb]") as "[Hctx Hmt]" => //. { iFrame. }
+  iMod (Hwp with "Hmt [Hfm]") as "Hmains". {
+    rewrite /f => {f Hwp Hnew}.
     iInduction (fns) as [] "IH" using map_ind => //.
     iApply big_sepM_insert => //. rewrite to_fntbl_insert.
     rewrite (insert_singleton_op); last by apply lookup_to_fntbl_None.
@@ -111,7 +96,7 @@ Proof.
   }
 
   iModIntro. iExists NotStuck, _, (replicate (length thread_mains) (λ _, True%I)), _.
-  iSplitL "Hh Hb Hf"; last first. 1: iSplitL.
+  iSplitL "Hctx"; last first. 1: iSplitL.
   - rewrite big_sepL2_fmap_l. iApply big_sepL2_replicate_2. iApply (big_sepL_impl with "Hmains").
     iIntros "!#" (? main ?); iDestruct 1 as (P) "[Hmain HP]".
     iApply wp_to_typed_stmt => //.
@@ -125,84 +110,6 @@ Proof.
 Qed.
 
 (** * Helper functions for using the adequacy lemma *)
-Definition block_to_loc (l: alloc_id): loc := (l, 0%Z).
-
-Definition block_list_to_loc (l: alloc_id): list mbyte → gmap loc mbyte :=
-  list_to_map ∘ imap (λ i b, (block_to_loc l +ₗ i, b)).
-
-Lemma block_list_to_loc_nil l :
-  block_list_to_loc l [] = ∅.
-Proof. done. Qed.
-
-Lemma block_list_to_loc_app l bs x :
-  block_list_to_loc l (bs ++ [x]) =
-  <[block_to_loc l +ₗ length bs:=x]> (block_list_to_loc l bs).
-Proof.
-  rewrite /block_list_to_loc /= -list_to_map_cons.
-  apply list_to_map_proper; first by apply imap_fst_NoDup, _.
-  rewrite imap_app /= -plus_n_O.
-    by symmetry; apply Permutation_cons_append.
-Qed.
-
-Lemma block_list_to_loc_comm j1 j2 z1 z2 y:
-  j1 ≠ j2 →
-  block_list_to_loc j1 z1 ∪ (block_list_to_loc j2 z2 ∪ y) =
-  block_list_to_loc j2 z2 ∪ (block_list_to_loc j1 z1 ∪ y).
-Proof.
-  move => Hneq. rewrite !assoc. f_equal. apply map_union_comm.
-  apply/map_disjoint_list_to_map_l/Forall_forall => -[??] Hin1.
-  apply not_elem_of_list_to_map_1 => /= Hin2. set_solver.
-Qed.
-
-Definition heap_list_to_heap : gmap alloc_id (list mbyte) → gmap loc mbyte :=
-  map_fold (λ b ls m, block_list_to_loc b ls ∪ m) ∅.
-
-Definition heap_list_to_allocs : gmap alloc_id (list mbyte) → allocs :=
-    fmap (λ l, to_allocation 0 (length l)).
-
-Lemma heap_list_to_heap_insert `{!refinedcG Σ} l v h :
-  h !! l = None →
-  ([∗ map] k↦qs ∈ heap_list_to_heap (<[l := v]> h), heap_mapsto_mbyte k 1 qs) -∗
-  ([∗ map] k↦qs ∈ heap_list_to_allocs (<[l := v]> h), allocs_entry k qs) -∗
-  block_to_loc l ↦ v ∗
-  ([∗ map] k↦qs ∈ heap_list_to_heap h, heap_mapsto_mbyte k 1 qs) ∗
-  ([∗ map] k↦qs ∈ heap_list_to_allocs h, allocs_entry k qs).
-Proof.
-  iIntros (HNone) "Hm Ha".
-  rewrite /heap_list_to_heap map_fold_insert_L //; last by move => *; apply block_list_to_loc_comm.
-  rewrite big_sepM_union. 2: {
-    apply/map_disjoint_list_to_map_l/Forall_forall => *.
-    induction h using map_ind => //.
-    move: HNone => /lookup_insert_None [??].
-    rewrite map_fold_insert_L //; last by move => *; apply block_list_to_loc_comm.
-    apply lookup_union_None. split; last by eauto.
-    apply not_elem_of_list_to_map_1. set_solver.
-  }
-  iDestruct "Hm" as "[Hv $]".
-  rewrite /heap_list_to_allocs fmap_insert big_sepM_insert; last by rewrite lookup_fmap HNone.
-  iDestruct "Ha" as "[Ha $]".
-  rewrite heap_mapsto_eq/heap_mapsto_def.
-  iSplitL "Ha". { iApply allocs_entry_to_loc_in_bounds => //. simpl. lia. }
-  iInduction (v) as [] "IH" using rev_ind => //.
-  rewrite block_list_to_loc_app big_sepM_insert ?big_sepL_app /= ?Nat.add_0_r.
-  + iDestruct "Hv" as "[$ Hl]". by iApply "IH".
-  + apply not_elem_of_list_to_map_1. set_unfold.
-    move => [[??][?[?[?[?/(lookup_lt_Some _ _ _) ?]]]]]. naive_solver lia.
-Qed.
-
-Lemma heap_list_blocks_agree fns gs:
-  blocks_used_agree (initial_state fns (heap_list_to_heap gs) (heap_list_to_allocs gs)).(st_heap) (initial_state fns (heap_list_to_heap gs) (heap_list_to_allocs gs)).(st_allocs).
-Proof.
-  move => /= l. rewrite /heap_list_to_allocs lookup_fmap fmap_None. move => Hgs i.
-  rewrite lookup_fmap fmap_None /heap_list_to_heap. move: Hgs.
-  induction gs as [|] using map_ind. { by rewrite map_fold_empty. }
-  rewrite map_fold_insert_L //; last by move => *; apply block_list_to_loc_comm.
-  move => /lookup_insert_None[??]. apply/lookup_union_None. split; [ | naive_solver ].
-  rewrite /block_list_to_loc /= not_elem_of_list_to_map_1 //.
-  move => /elem_of_list_fmap[[??]/=[?]] /(elem_of_lookup_imap_1 _ _ _)[? [?[??]]].
-  simplify_eq.
-Qed.
-
 Definition fn_lists_to_fns (locs : list loc) (fns : list function) : gmap loc function :=
   list_to_map (zip locs fns).
 
